theories/simulations/isim/ITactics.v
@@ -9,7 +9,7 @@ Require Export ITacticsCore.
 
 Ltac init_sim :=
   first [eapply hmod_sim_reflR | econs];
-  [i; s; repeat unfold_hmod; s
+  [i; s; (hrepeat do 1 unfold_hmod); s
   |eauto
   |try prove_sub_perm
   |try prove_sub_perm
